theories/lang/adequacy.v
@@ -4,13 +4,13 @@ From lrust.lang Require Export heap.
 From lrust.lang Require Import proofmode notation.
 
 Class heapPreG Σ := HeapPreG {
-  heap_preG_iris :> irisPreG lrust_lang Σ;
+  heap_preG_ownP :> ownPPreG lrust_lang Σ;
   heap_preG_heap :> inG Σ (authR heapUR);
   heap_preG_heap_freeable :> inG Σ (authR heap_freeableUR)
 }.
 
 Definition heapΣ : gFunctors :=
-  #[irisΣ state;
+  #[ownPΣ state;
     GFunctor (constRF (authR heapUR));
     GFunctor (constRF (authR heap_freeableUR))].
 Instance subG_heapPreG {Σ} : subG heapΣ Σ → heapPreG Σ.
@@ -20,7 +20,7 @@ Definition heap_adequacy Σ `{heapPreG Σ} e σ φ :
   (∀ `{heapG Σ}, {{ heap_ctx }} e {{ v, ⌜φ v⌝ }}) →
   adequate e σ φ.
 Proof.
-  intros Hwp; eapply (wp_adequacy Σ). iIntros (?) "Hσ".
+  intros Hwp; eapply (ownP_adequacy Σ _). iIntros (?) "Hσ".
   iMod (own_alloc (● to_heap σ)) as (vγ) "Hvγ".
   { apply (auth_auth_valid (to_heap _)), to_heap_valid. }
   iMod (own_alloc (● (∅ : heap_freeableUR))) as (fγ) "Hfγ"; first done.
