theories/lang/lifting.v
@@ -1,4 +1,4 @@
-From iris.program_logic Require Export weakestpre.
+From iris.program_logic Require Export weakestpre ownp.
 From iris.program_logic Require Import ectx_lifting.
 From lrust.lang Require Export lang.
 From lrust.lang Require Import tactics.
@@ -6,8 +6,10 @@ From iris.proofmode Require Import tactics.
 Import uPred.
 Local Hint Extern 0 (head_reducible _ _) => do_head_step eauto 2.
 
+(* TODO : as for heap_lang, directly use a global heap invariant. *)
+
 Section lifting.
-Context `{irisG lrust_lang Σ}.
+Context `{ownPG lrust_lang Σ}.
 Implicit Types P Q : iProp Σ.
 Implicit Types ef : option expr.
 
@@ -30,7 +32,7 @@ Lemma wp_alloc_pst E σ n:
       ⌜∃ vl, n = length vl ∧ init_mem l vl σ = σ'⌝ ∗
       ownP σ' }}}.
 Proof.
-  iIntros (? Φ) "HP HΦ". iApply (wp_lift_atomic_head_step _ σ); eauto.
+  iIntros (? Φ) "HP HΦ". iApply (ownP_lift_atomic_head_step _ σ); eauto.
   iFrame "HP". iNext. iIntros (v2 σ2 ef) "% HP". inv_head_step.
   rewrite big_sepL_nil right_id. by iApply "HΦ"; iFrame; eauto.
 Qed.
@@ -41,7 +43,7 @@ Lemma wp_free_pst E σ l n :
   {{{ ▷ ownP σ }}} Free (Lit $ LitInt n) (Lit $ LitLoc l) @ E
   {{{ RET LitV $ LitUnit; ownP (free_mem l (Z.to_nat n) σ) }}}.
 Proof.
-  iIntros (???)  "HP HΦ". iApply (wp_lift_atomic_head_step _ σ); eauto.
+  iIntros (???)  "HP HΦ". iApply (ownP_lift_atomic_head_step _ σ); eauto.
   iFrame "HP". iNext. iIntros (v2 σ2 ef) "% HP". inv_head_step.
   rewrite big_sepL_nil right_id. by iApply "HΦ".
 Qed.
@@ -50,7 +52,7 @@ Lemma wp_read_sc_pst E σ l n v :
   σ !! l = Some (RSt n, v) →
   {{{ ▷ ownP σ }}} Read ScOrd (Lit $ LitLoc l) @ E {{{ RET v; ownP σ }}}.
 Proof.
-  iIntros (??) "?HΦ". iApply wp_lift_atomic_det_head_step; eauto.
+  iIntros (??) "?HΦ". iApply ownP_lift_atomic_det_head_step; eauto.
   by intros; inv_head_step; eauto using to_of_val.
   rewrite big_sepL_nil right_id; iFrame.
 Qed.
@@ -60,7 +62,7 @@ Lemma wp_read_na2_pst E σ l n v :
   {{{ ▷ ownP σ }}} Read Na2Ord (Lit $ LitLoc l) @ E
   {{{ RET v; ownP (<[l:=(RSt n, v)]>σ) }}}.
 Proof.
-  iIntros (??) "?HΦ". iApply wp_lift_atomic_det_head_step; eauto.
+  iIntros (??) "?HΦ". iApply ownP_lift_atomic_det_head_step; eauto.
   by intros; inv_head_step; eauto using to_of_val.
   rewrite big_sepL_nil right_id; iFrame.
 Qed.
@@ -72,7 +74,7 @@ Lemma wp_read_na1_pst E l Φ :
           WP Read Na2Ord (Lit $ LitLoc l) @ E {{ Φ }})) -∗
   WP Read Na1Ord (Lit $ LitLoc l) @ E {{ Φ }}.
 Proof.
-  iIntros "HΦP". iApply (wp_lift_head_step E); auto.
+  iIntros "HΦP". iApply (ownP_lift_head_step E); auto.
   iMod "HΦP" as (σ n v) "(%&HΦ&HP)". iModIntro. iExists σ. iSplit. done. iFrame.
   iNext. iIntros (e2 σ2 ef) "% HΦ". inv_head_step.
   rewrite big_sepL_nil right_id. iApply ("HP" with "HΦ").
@@ -83,7 +85,7 @@ Lemma wp_write_sc_pst E σ l v v' :
   {{{ ▷ ownP σ }}} Write ScOrd (Lit $ LitLoc l) (of_val v) @ E
   {{{ RET LitV LitUnit; ownP (<[l:=(RSt 0, v)]>σ) }}}.
 Proof.
-  iIntros (??) "?HΦ". iApply wp_lift_atomic_det_head_step; eauto.
+  iIntros (??) "?HΦ". iApply ownP_lift_atomic_det_head_step; eauto.
   by intros; inv_head_step; eauto. rewrite big_sepL_nil right_id; iFrame.
 Qed.
 
@@ -92,7 +94,7 @@ Lemma wp_write_na2_pst E σ l v v' :
   {{{ ▷ ownP σ }}} Write Na2Ord (Lit $ LitLoc l) (of_val v) @ E
   {{{ RET LitV LitUnit; ownP (<[l:=(RSt 0, v)]>σ) }}}.
 Proof.
-  iIntros (??) "?HΦ". iApply wp_lift_atomic_det_head_step; eauto.
+  iIntros (??) "?HΦ". iApply ownP_lift_atomic_det_head_step; eauto.
   by intros; inv_head_step; eauto. rewrite big_sepL_nil right_id; iFrame.
 Qed.
 
@@ -103,7 +105,7 @@ Lemma wp_write_na1_pst E l v Φ :
        WP Write Na2Ord (Lit $ LitLoc l) (of_val v) @ E {{ Φ }})) -∗
   WP Write Na1Ord (Lit $ LitLoc l) (of_val v) @ E {{ Φ }}.
 Proof.
-  iIntros "HΦP". iApply (wp_lift_head_step E); auto.
+  iIntros "HΦP". iApply (ownP_lift_head_step E); auto.
   iMod "HΦP" as (σ v') "(%&HΦ&HP)". iModIntro. iExists σ. iSplit. done. iFrame.
   iNext. iIntros (e2 σ2 ef) "% HΦ". inv_head_step.
   rewrite big_sepL_nil right_id. iApply ("HP" with "HΦ").
@@ -120,7 +122,7 @@ Lemma wp_cas_pst E n σ l e1 lit1 lit2 litl :
       else ⌜lit_neq σ lit1 litl⌝ ∗ ownP σ }}}.
 Proof.
   iIntros (?%of_to_val ? Hdec Hn ?) "HP HΦ". subst.
-  iApply wp_lift_atomic_head_step; eauto.
+  iApply ownP_lift_atomic_head_step; eauto.
   { destruct Hdec as [Heq|Hneq].
     - specialize (Hn Heq). subst. do 3 eexists. by eapply CasSucS.
     - do 3 eexists. by eapply CasFailS. }
@@ -135,7 +137,7 @@ Qed.
 Lemma wp_fork E e :
   {{{ ▷ WP e {{ _, True }} }}} Fork e @ E {{{ RET LitV LitUnit; True }}}.
 Proof.
-  iIntros (?) "?HΦ". iApply wp_lift_pure_det_head_step; eauto.
+  iIntros (?) "?HΦ". iApply ownP_lift_pure_det_head_step; eauto.
   by intros; inv_head_step; eauto. iNext.
   rewrite big_sepL_singleton. iFrame. iApply wp_value. done. by iApply "HΦ".
 Qed.
@@ -148,7 +150,7 @@ Lemma wp_rec E e f xl erec erec' el Φ :
   ▷ WP subst' f e erec' @ E {{ Φ }} -∗
   WP App e el @ E {{ Φ }}.
 Proof.
-  iIntros (-> ???) "?". iApply wp_lift_pure_det_head_step; subst; eauto.
+  iIntros (-> ???) "?". iApply ownP_lift_pure_det_head_step; subst; eauto.
   by intros; inv_head_step; eauto. iNext. rewrite big_sepL_nil. by iFrame.
 Qed.
 
@@ -157,8 +159,8 @@ Lemma wp_bin_op_heap E σ op l1 l2 l' :
   {{{ ▷ ownP σ }}} BinOp op (Lit l1) (Lit l2) @ E
   {{{ l'', RET LitV l''; ⌜bin_op_eval σ op l1 l2 l''⌝ ∗ ownP σ }}}.
 Proof.
-  iIntros (? Φ) "HP HΦ". iApply wp_lift_atomic_head_step; eauto.
-  iFrame "HP". iNext. iIntros (e2 σ2 efs Hs) "Ho". 
+  iIntros (? Φ) "HP HΦ". iApply ownP_lift_atomic_head_step; eauto.
+  iFrame "HP". iNext. iIntros (e2 σ2 efs Hs) "Ho".
   inv_head_step; rewrite big_sepL_nil right_id.
   iApply "HΦ". eauto.
 Qed.
@@ -168,9 +170,9 @@ Lemma wp_bin_op_pure E op l1 l2 l' :
   {{{ True }}} BinOp op (Lit l1) (Lit l2) @ E
   {{{ l'' σ, RET LitV l''; ⌜bin_op_eval σ op l1 l2 l''⌝ }}}.
 Proof.
-  iIntros (? Φ) "HΦ". iApply wp_lift_pure_head_step; eauto.
+  iIntros (? Φ) "HΦ". iApply ownP_lift_pure_head_step; eauto.
   { intros. inv_head_step. done. }
-  iNext. iIntros (e2 efs σ Hs). 
+  iNext. iIntros (e2 efs σ Hs).
   inv_head_step; rewrite big_sepL_nil right_id.
   rewrite -wp_value //. iApply "HΦ". eauto.
 Qed.
@@ -180,7 +182,7 @@ Lemma wp_case E i e el Φ :
   nth_error el (Z.to_nat i) = Some e →
   ▷ WP e @ E {{ Φ }} -∗ WP Case (Lit $ LitInt i) el @ E {{ Φ }}.
 Proof.
-  iIntros (??) "?". iApply wp_lift_pure_det_head_step; eauto.
+  iIntros (??) "?". iApply ownP_lift_pure_det_head_step; eauto.
   by intros; inv_head_step; eauto. iNext. rewrite big_sepL_nil. by iFrame.
 Qed.
 End lifting.
