theories/typing/type_context.v
@@ -1,0 +1,115 @@
+From iris.proofmode Require Import tactics.
+From iris.base_logic Require Import big_op.
+From lrust.lang Require Import notation.
+From lrust.lifetime Require Import definitions.
+From lrust.typing Require Import type lft_contexts.
+
+Section type_context.
+  Context `{typeG Σ}.
+
+  Definition path := expr.
+
+  Fixpoint eval_path (ν : path) : option val :=
+    match ν with
+    | BinOp OffsetOp e (Lit (LitInt n)) =>
+      match eval_path e with
+      | Some (#(LitLoc l)) => Some (#(shift_loc l n))
+      | _ => None
+      end
+    | e => to_val e
+    end.
+
+  Inductive tctx_elt : Type :=
+  | TCtx_holds (p : path) (ty : type)
+  | TCtx_guarded (p : path) (κ : lft) (ty : type).
+  Definition tctx := list tctx_elt.
+
+  Definition tctx_elt_interp (tid : thread_id) (x : tctx_elt) : iProp Σ :=
+    match x with
+    | TCtx_holds p ty => ∃ v, ⌜eval_path p = Some v⌝ ∗ ty.(ty_own) tid [v]
+    | TCtx_guarded p κ ty => ∃ v, ⌜eval_path p = Some v⌝ ∗
+        ∀ E, ⌜↑lftN ⊆ E⌝ -∗ [†κ] ={E}=∗ ▷ ty.(ty_own) tid [v]
+    end%I.
+  Definition tctx_interp (tid : thread_id) (T : tctx) : iProp Σ :=
+    ([∗ list] x ∈ T, tctx_elt_interp tid x)%I.
+
+  Global Instance tctx_interp_permut:
+    Proper (eq ==> (≡ₚ) ==> (⊣⊢)) tctx_interp.
+  Proof. intros ?? -> ???. by apply big_opL_permutation. Qed.
+
+  Definition tctx_incl (E : lectx) (L : llctx) (T1 T2 : tctx): Prop :=
+    ∀ qE qL, lft_ctx -∗ lectx_interp E qE -∗ llctx_interp L qL -∗
+          □ ∀ tid, tctx_interp tid T1 -∗ tctx_interp tid T2.
+
+  Global Instance tctx_incl_preorder E L : PreOrder (tctx_incl E L).
+  Proof.
+    split.
+    - by iIntros (???) "_ _ _ !# * $".
+    - iIntros (??? H1 H2 ??) "#LFT HE HL".
+      iDestruct (H1 with "LFT HE HL") as "#H1".
+      iDestruct (H2 with "LFT HE HL") as "#H2".
+      iIntros "{HE HL}!# * H". iApply "H2". by iApply "H1".
+  Qed.
+
+  Lemma contains_tctx_incl E L T1 T2 : T1 `contains` T2 → tctx_incl E L T2 T1.
+  Proof.
+    rewrite /tctx_incl. iIntros (EQ ??) "_ _ _ !# * H". by iApply big_sepL_contains.
+  Qed.
+
+  Lemma tctx_incl_frame E L T T1 T2 :
+    tctx_incl E L T2 T1 → tctx_incl E L (T++T2) (T++T1).
+  Proof.
+    iIntros (Hincl ??) "#LFT HE HL". rewrite /tctx_interp.
+    iDestruct (Hincl with "LFT HE HL") as"#Hincl".
+    iIntros "{HE HL} !# *". rewrite !big_sepL_app.
+    iIntros "[$ ?]". by iApply "Hincl".
+  Qed.
+
+  Lemma copy_tctx_incl E L p `(!Copy ty) :
+    tctx_incl E L [TCtx_holds p ty] [TCtx_holds p ty; TCtx_holds p ty].
+  Proof.
+    iIntros (??) "_ _ _ !# *". rewrite /tctx_interp !big_sepL_cons big_sepL_nil.
+    by iIntros "[#$ $]".
+  Qed.
+
+  Lemma subtype_tctx_incl E L p ty1 ty2 :
+    subtype E L ty1 ty2 → tctx_incl E L [TCtx_holds p ty1] [TCtx_holds p ty2].
+  Proof.
+    iIntros (Hst ??) "#LFT HE HL".
+    iDestruct (subtype_own _ _ _ _ Hst with "LFT HE HL") as "#Hst".
+    iIntros "{HE HL} !# * H". rewrite /tctx_interp !big_sepL_singleton /=.
+    iDestruct "H" as (v) "[% H]". iExists _. iFrame "%". by iApply "Hst".
+  Qed.
+
+  Definition deguard_tctx_elt κ x :=
+    match x with
+    | TCtx_guarded p κ' ty =>
+      if decide (κ = κ') then TCtx_holds p ty else x
+    | _ => x
+    end.
+
+  Lemma deguard_tctx_elt_interp tid E κ x :
+    ↑lftN ⊆ E → [†κ] -∗ tctx_elt_interp tid x ={E}=∗
+        ▷ tctx_elt_interp tid (deguard_tctx_elt κ x).
+  Proof.
+    iIntros (?) "H† H". destruct x as [|? κ' ?]; simpl. by auto.
+    destruct (decide (κ = κ')) as [->|]; simpl; last by auto.
+    iDestruct "H" as (v) "[% H]". iExists v. iSplitR. by auto.
+    by iApply ("H" with "[] H†").
+  Qed.
+
+  Definition deguard_tctx κ (T : tctx) : tctx :=
+    deguard_tctx_elt κ <$> T.
+
+  Lemma deguard_tctx_interp tid E κ T :
+    ↑lftN ⊆ E → [†κ] -∗ tctx_interp tid T ={E}=∗
+        ▷ tctx_interp tid (deguard_tctx κ T).
+  Proof.
+    iIntros (?) "#H† H". rewrite /tctx_interp big_sepL_fmap.
+    iApply (big_opL_forall (λ P Q, [†κ] -∗ P ={E}=∗ ▷ Q) with "H† H").
+    { by iIntros (?) "_ $". }
+    { iIntros (?? A ?? B) "#H† [H1 H2]". iSplitL "H1".
+        by iApply (A with "H†"). by iApply (B with "H†"). }
+    move=>/= _ ? _. by apply deguard_tctx_elt_interp.
+  Qed.
+End type_context.
